a working draft

chapter04/demos/leader_election_work.dfy
@@ -10,6 +10,7 @@ datatype Constants = Constants(ids: seq<nat>) {
 
   predicate WF() {
     && 0 < |ids|
+    && UniqueIds()
   }
 }
 
@@ -39,7 +40,8 @@ function NextIdx(k: Constants, idx: nat) : nat
   requires k.WF()
   requires k.ValidIdx(idx)
 {
-  (idx + 1) % |k.ids|
+  //(idx + 1) % |k.ids|
+  if idx + 1 == |k.ids| then 0 else idx + 1
 }
 
 predicate Transmission(k: Constants, v: Variables, v': Variables, src: nat)
@@ -59,7 +61,7 @@ predicate Transmission(k: Constants, v: Variables, v': Variables, src: nat)
   && var dst_new_max := max(v.highest_heard[dst], message);
   // XXX Manos: How could this have been a bug!? How could a src, having sent message X, ever send message Y < X!?
 
-  && v' == v.(highest_heard := v.highest_heard[dst := message])
+  && v' == v.(highest_heard := v.highest_heard[dst := dst_new_max])
 }
 
 datatype Step = TransmissionStep(src: nat)
@@ -99,10 +101,73 @@ predicate Safety(k: Constants, v: Variables)
 // Proof
 //////////////////////////////////////////////////////////////////////////////
 
+// // accounting for wrap
+// // start, end exclusive.
+// predicate Between(start: nat, i: nat, end: nat)
+// {
+//   if start<end
+//   then start<i<end
+//   else i<end || start<i
+// }
+// 
+// predicate IsChord(k: Constants, v: Variables, start: nat, end: nat)
+// {
+//   && k.WF()
+//   && v.WF(k)
+//   && k.ValidIdx(start)
+//   && k.ValidIdx(end)
+//   && k.ids[start] == v.highest_heard[end]
+// }
+// 
+// predicate OnChordHeardDominatesId(k: Constants, v: Variables, start: nat, end: nat)
+//   requires k.WF()
+//   requires v.WF(k)
+// {
+//   forall i:nat | k.ValidIdx(i) && Between(start, i, end) :: v.highest_heard[i] > k.ids[i]
+// }
+// 
+// predicate OnChordHeardDominatesIdInv(k: Constants, v: Variables)
+//   requires k.WF()
+//   requires v.WF(k)
+// {
+//   forall start:nat, end:nat | k.ValidIdx(start) && k.ValidIdx(end) && IsChord(k, v, start, end) :: OnChordHeardDominatesId(k, v, start, end)
+// }
+
+predicate Between(k: Constants, startExclusive: nat, i: nat, endExclusive: nat)
+{
+  if startExclusive < endExclusive
+  then
+    startExclusive < i < endExclusive
+  else
+    startExclusive < i || i < endExclusive
+}
+
+predicate IsChord(k: Constants, v: Variables, start: nat, end: nat)
+{
+  && k.WF()
+  && v.WF(k)
+  && k.ValidIdx(start)
+  && k.ValidIdx(end)
+  && k.ids[start] == v.highest_heard[end]
+}
+predicate HeardOnChordDominatesID(k: Constants, v: Variables, start: nat, end: nat)
+{
+  IsChord(k, v, start, end)
+  ==> (forall i:nat | k.ValidIdx(i) && Between(k, start, i, end) :: v.highest_heard[i] > k.ids[i])
+}
+
+predicate HeardDominatesInv(k: Constants, v: Variables)
+{
+  && (forall start, end | k.ValidIdx(start) && k.ValidIdx(end) :: HeardOnChordDominatesID(k, v, start, end))
+}
+
+
 predicate Inv(k: Constants, v: Variables)
 {
   && k.WF()
   && v.WF(k)
+//  && OnChordHeardDominatesIdInv(k, v)
+  && HeardDominatesInv(k, v)
   && Safety(k, v)
 }
 
@@ -117,6 +182,58 @@ lemma NextPreservesInv(k: Constants, v: Variables, v': Variables)
   requires Next(k, v, v')
   ensures Inv(k, v')
 {
+  assert exists step :: NextStep(k, v, v', step);
+  var step :| NextStep(k, v, v', step);
+  var src := step.src;
+  var dst := NextIdx(k, src);
+  assert Transmission(k, v, v', src);
+  forall start:nat, end:nat | k.ValidIdx(start) && k.ValidIdx(end) ensures HeardOnChordDominatesID(k, v', start, end)
+  {
+    var message := max(v.highest_heard[src], k.ids[src]);
+    var dst_new_max := max(v.highest_heard[dst], message);
+
+    if IsChord(k, v', start, end) {
+      forall i:nat | k.ValidIdx(i) && Between(k, start, i, end)
+        ensures v'.highest_heard[i] > k.ids[i]
+      {
+        if dst==end {
+          // which of the three values did highest_heard[dst] take on?
+          if v'.highest_heard[dst] == v.highest_heard[dst] {
+            assert v'.highest_heard[i] > k.ids[i];
+          } else if v'.highest_heard[dst] == k.ids[src] {
+            calc {
+              k.ids[src];
+                // this branch
+              == v'.highest_heard[dst];
+                // IsChord
+              == k.ids[start];
+            }
+            assert src!=start;
+            assert k.UniqueIds(); // WTF
+            assert v'.highest_heard[i] > k.ids[i];
+          } else {
+//            if i==src {
+//              assert v.highest_heard[i] > k.ids[i];
+//              assert v'.highest_heard[i] > k.ids[i];
+//            } else {
+//              assert Between(k, start, i, src);
+//              assert v'.highest_heard[i] > k.ids[i];
+//            }
+            assert v'.highest_heard[i] > k.ids[i];
+          }
+        } else if dst==start {
+          assert v'.highest_heard[i] > k.ids[i];
+        } else if Between(k, start, dst, end) {
+          assert v'.highest_heard[i] > k.ids[i];
+        } else if Between(k, end, dst, start) {
+          assert v'.highest_heard[i] > k.ids[i];
+        } else {
+          assert false;
+        }
+      }
+      assert HeardOnChordDominatesID(k, v', start, end);
+    }
+  }
 }
 
 lemma InvImpliesSafety(k: Constants, v: Variables)
