chapter04/demos/leader_election_instructor_script.md
@@ -29,6 +29,98 @@ docker container run -t -i --mount src="`pwd`",target=/home/dafnyserver/work,typ
 
 - fix the type inference failures on nat
 - in my test run, it got really slow. Add /timeLimit:20
+- break out the profiler:
+  ```../../tools/dafny-profile.py 20 "*NextPreservesInv" leader_election_work.dfy```
+  - huh, no frequent quantifier instantiations
+
+(voodoo) So we try noNLarith to see if Z3 is getting hung up on nonlinear algebraic reductions.
+Yep, now it fails quickly.
+Where do we have nonlinear arithmetic? Ugh, that mod. We don't really need mod here,
+so instead of teaching you how to manage mod, let's just bail on it.
+
+(BUG #1 was "idx + 0", but I'm not going to re-introduce that one.)
+
+So time to dig into the broken proof.
+* Choose a step. (get through the exists, skolemize the step choice & params)
+
+XXX does the inductive invariant lesson preced this one?
+...wait, why would this even work? Safety is like the manhole: a good property, but not
+inductive. Lots of system states that are a step away from Safety but shouldn't be
+reachable.
+It's time to ask *why* should the system work? What's the key intuition?
+The answer is in the animation: As "big" identifiers work around the ring, they
+build "chords" from their origin to the farthest point they've reached.
+Sometimes one chord will gobble up another's head, breaking it, but anytime there is a
+chord, all the nodes it has passed over have heard about it and are dominated by it.
+The biggest ID's chord never gets gobbled; eventually it reaches all the way around the ring.
+
+Type out IsChord, OnChordHeardDominatesId.
+
+Cheat sheet:
+```
+  predicate Between(start: nat, i: nat, end: nat)
+  {
+    if start<end
+    then start<i<end
+    else i<end || start<i
+  }
+
+  predicate IsChord(k: Constants, v: Variables, start: nat, end: nat)
+  {
+    && k.WF()
+    && v.WF(k)
+    && k.ValidIdx(start)
+    && k.ValidIdx(end)
+    && k.ids[start] == v.highest_heard[end]
+  }
+
+  predicate OnChordHeardDominatesId(k: Constants, v: Variables, start: nat, end: nat)
+    requires k.WF()
+    requires v.WF(k)
+  {
+    forall i:nat | k.ValidIdx(i) && Between(start, i, end) :: v.highest_heard[i] > k.ids[i]
+  }
+
+  predicate OnChordHeardDominatesIdInv(k: Constants, v: Variables)
+    requires k.WF()
+    requires v.WF(k)
+  {
+    forall start:nat, end:nat | k.ValidIdx(start) && k.ValidIdx(end) && IsChord(k, v, start, end) :: OnChordHeardDominatesId(k, v, start, end)
+  }
+```
+
+Proof sketch:
+If we are gonna violate Safety, we'll need two idxes i, j that both think they're
+leader. WOLOG let i be the one with the larger id. It is leader, so IsChord(k,v,i,i).
+So every *other* node, including j is Between(k, i, j, i), so
+v.highest_heard[j] > k.ids[j], which is a contradiction with IsLeader(j).
+
+...need to define Between.
+Could require k.ValidIdx on all args, but meh, don't need to.
+Note that start and end are exclusive:
+* Since the start doesn't adjust its own highest_heard based on its own id, it's not
+  affected by the message traveling along the chord.
+* Since end can be equal to start when the chord completes the ring, we don't want to
+  include it, since it *won't* have highest_heard > id.
+** name inductive predicate, use ValidIdx
+
+Try to nail down Safety first.
+  -- try the contradiction above; punchline is a trigger OnChordHeardDominatesId
+
+Use a case analysis on dst
+  - discrete cases first, then Betweens -- dafny seems to do better.
+    { dst==end, dst==start, Between(start,dst,end), Between(end,dst,start), false }
+  - in dst==end case, split on which thing was max,
+      { v'.highest_heard[dst] == v.highest_heard[dst],
+        v'.highest_heard[dst] == k.ids[src],
+        v'.highest_heard[dst] == v.highest_heard[src] }
+    # FIX discover (in else branch) that we screwed up the assignment, ignoring dst_new_max
+    # in middle branch (k.ids[src]), assert:
+      k.ids[src] == v'.highest_heard[dst] // this branch
+      v'.highest_heard[dst] == k.ids[start] // IsChord
+      assert src!=start // no idea why XXX-TODO
+      assert k.UniqueIds() // WTF -- FIX by adding to Constants.WF
+...now the proof goes through.
 
 
 ***
